add three lemmas to transform.dfy

logics/Transform.dfy
@@ -4,9 +4,7 @@ module Transform {
 
   import opened Setups
 
-  // ============================================================
-  // 1. Basic transformations
-  // ============================================================
+  //  ----------------reverse-----------------
 
   // Reverse one row
   function ReverseRow(row: seq<int>): seq<int>
@@ -28,22 +26,9 @@ module Transform {
     seq(N, i requires 0 <= i < N => ReverseRow(grid[i]))
   }
 
-  // Transpose grid
-  function Transpose(grid: Grid): Grid
-    requires ValidGrid(grid)
-    ensures ValidGrid(Transpose(grid))
-    ensures forall i, j ::
-              0 <= i < N && 0 <= j < N ==>
-                Transpose(grid)[i][j] == grid[j][i]
-  {
-    seq(N, i requires 0 <= i < N =>
-      seq(N, j requires 0 <= j < N => grid[j][i]))
-  }
 
-  // ============================================================
-  // 2. Property-preservation lemmas
-  // ============================================================
 
+  // 2. Property-preservation lemmas for reverse
   lemma ReversePreservesValues(grid: Grid)
     requires ValidGrid(grid)
     requires ValidValues(grid)
@@ -57,17 +42,6 @@ module Transform {
     }
   }
 
-  lemma TransposePreservesValues(grid: Grid)
-    requires ValidGrid(grid)
-    requires ValidValues(grid)
-    ensures ValidValues(Transpose(grid))
-  {
-    forall i, j | 0 <= i < N && 0 <= j < N
-      ensures Transpose(grid)[i][j] == 0 || IsPowerOfTwo(Transpose(grid)[i][j])
-    {
-      assert Transpose(grid)[i][j] == grid[j][i];
-    }
-  }
 
   lemma ReversePreservesWin(grid: Grid)
     requires ValidGrid(grid)
@@ -89,24 +63,6 @@ module Transform {
     }
   }
 
-  lemma TransposePreservesWin(grid: Grid)
-    requires ValidGrid(grid)
-    requires ValidValues(grid)
-    ensures HasWinTile(grid) == HasWinTile(Transpose(grid))
-  {
-    if HasWinTile(grid) {
-      var i, j :| 0 <= i < N && 0 <= j < N && grid[i][j] == 2048;
-      assert Transpose(grid)[j][i] == grid[i][j];
-      assert exists ii, jj :: 0 <= ii < N && 0 <= jj < N && Transpose(grid)[ii][jj] == 2048;
-    }
-
-    if HasWinTile(Transpose(grid)) {
-      var i, j :| 0 <= i < N && 0 <= j < N && Transpose(grid)[i][j] == 2048;
-      assert Transpose(grid)[i][j] == grid[j][i];
-      assert grid[j][i] == 2048;
-      assert exists ii, jj :: 0 <= ii < N && 0 <= jj < N && grid[ii][jj] == 2048;
-    }
-  }
 
   lemma ReversePreservesEmpty(grid: Grid)
     requires ValidGrid(grid)
@@ -128,195 +84,182 @@ module Transform {
     }
   }
 
-  lemma TransposePreservesEmpty(grid: Grid)
+
+  lemma EnsuresMoreToMerge(grid: Grid)
     requires ValidGrid(grid)
     requires ValidValues(grid)
-    ensures HasEmptyTile(grid) == HasEmptyTile(Transpose(grid))
+    requires MoreToMerge(grid)
+    ensures
+      (exists i, j ::
+         0 <= i < N &&
+         0 <= j < N - 1 &&
+         grid[i][j] == grid[i][j + 1])
+      ||
+      (exists i, j ::
+         0 <= i < N - 1 &&
+         0 <= j < N &&
+         grid[i][j] == grid[i + 1][j])
   {
-    if HasEmptyTile(grid) {
-      var i, j :| 0 <= i < N && 0 <= j < N && grid[i][j] == 0;
-      assert Transpose(grid)[j][i] == 0;
-      assert exists ii, jj :: 0 <= ii < N && 0 <= jj < N && Transpose(grid)[ii][jj] == 0;
+  }
+
+  lemma ReverseGridAdjacent(grid: Grid, i: int, j: int)
+    requires ValidGrid(grid)
+    requires ValidValues(grid)
+    requires 0 <= i < N
+    requires 0 <= j < N-1
+    requires grid[i][j] == grid[i][j+1]
+    ensures Reverse(grid)[i][N-1-j] == Reverse(grid)[i][N-2-j]
+  {
+  }
+
+  lemma RemoveExist(grid: Grid) returns (i: int, j: int)
+    requires ValidGrid(grid)
+    requires ValidValues(grid)
+    requires exists i, j :: twotilesadjacent(i, j, grid)
+    ensures twotilesadjacent(i, j, grid)
+  {
+    var ii, jj :| twotilesadjacent(ii, jj, grid);
+    i, j := ii, jj;
+  }
+
+  lemma AddExist(grid: Grid, i: int, j: int)
+    requires ValidGrid(grid)
+    requires ValidValues(grid)
+    requires twotilesadjacent(i, j, grid)
+    ensures exists ii, jj :: twotilesadjacent(ii, jj, grid)
+  {
+  }
+
+  lemma ReversePreservesMoreToMerge(grid: Grid)
+    requires ValidGrid(grid)
+    requires ValidValues(grid)
+    ensures MoreToMerge(grid) == MoreToMerge(Reverse(grid))
+  {
+    // grid -> Reverse(grid)
+    if MoreToMerge(grid) {
+      if exists i, j ::
+          0 <= i < N && 0 <= j < N - 1 &&
+          grid[i][j] == grid[i][j + 1]
+      {
+        var i, j :|
+          0 <= i < N && 0 <= j < N - 1 &&
+          grid[i][j] == grid[i][j + 1];
+
+        assert 0 <= N - 2 - j < N - 1;
+        assert Reverse(grid)[i][N - 2 - j] == grid[i][j + 1];
+        assert Reverse(grid)[i][N - 1 - j] == grid[i][j];
+
+        assert exists ii, jj ::
+            ii == i &&
+            jj == N - 2 - j &&
+            0 <= ii < N &&
+            0 <= jj < N - 1 &&
+            Reverse(grid)[ii][jj] == Reverse(grid)[ii][jj + 1];
+      } else {
+        assert exists i, j {:trigger grid[i][j], grid[i + 1][j]} ::
+            0 <= i < N - 1 && 0 <= j < N &&
+            grid[i][j] == grid[i + 1][j];
+
+        var i, j :| 0 <= i < N - 1 && 0 <= j < N && grid[i][j] == grid[i + 1][j];
+
+        assert 0 <= N - 1 - j < N;
+        assert Reverse(grid)[i][N - 1 - j] == grid[i][j];
+        assert Reverse(grid)[i + 1][N - 1 - j] == grid[i + 1][j];
+
+        assert exists ii, jj {:trigger Reverse(grid)[ii][jj], Reverse(grid)[ii + 1][jj]} ::
+            ii == i &&
+            jj == N - 1 - j &&
+            0 <= ii < N - 1 &&
+            0 <= jj < N &&
+            Reverse(grid)[ii][jj] == Reverse(grid)[ii + 1][jj];
+      }
     }
 
-    if HasEmptyTile(Transpose(grid)) {
-      var i, j :| 0 <= i < N && 0 <= j < N && Transpose(grid)[i][j] == 0;
-      assert Transpose(grid)[i][j] == grid[j][i];
-      assert grid[j][i] == 0;
-      assert exists ii, jj :: 0 <= ii < N && 0 <= jj < N && grid[ii][jj] == 0;
+    // Reverse(grid) -> grid
+    if MoreToMerge(Reverse(grid)) {
+      if exists i, j ::
+          0 <= i < N && 0 <= j < N - 1 &&
+          Reverse(grid)[i][j] == Reverse(grid)[i][j + 1]
+      {
+        var i, j :|
+          0 <= i < N && 0 <= j < N - 1 &&
+          Reverse(grid)[i][j] == Reverse(grid)[i][j + 1];
+
+        assert 0 <= N - 2 - j < N - 1;
+        assert Reverse(grid)[i][j] == grid[i][N - 1 - j];
+        assert Reverse(grid)[i][j + 1] == grid[i][N - 2 - j];
+
+        assert exists ii, jj ::
+            ii == i &&
+            jj == N - 2 - j &&
+            0 <= ii < N &&
+            0 <= jj < N - 1 &&
+            grid[ii][jj] == grid[ii][jj + 1];
+      } else {
+        // assert exists i, j {:trigger Reverse(grid)[i][j], Reverse(grid)[i + 1][j]} ::
+        //     0 <= i < N - 1 && 0 <= j < N &&
+        //     Reverse(grid)[i][j] == Reverse(grid)[i + 1][j];
+        // assert exists i, j :: twotilesadjacent(i, j, grid);
+
+        assert exists i, j :: twotilesadjacent(i, j, Reverse(grid));
+        var i, j := ExistsVerticalMerge(Reverse(grid));
+        assert 0 <= N - 1 - j < N;
+        assert Reverse(grid)[i][j] == grid[i][N - 1 - j];
+        assert Reverse(grid)[i + 1][j] == grid[i + 1][N - 1 - j];
+
+        assert exists ii, jj {:trigger grid[ii][jj], grid[ii + 1][jj]} ::
+            ii == i &&
+            jj == N - 1 - j &&
+            0 <= ii < N - 1 &&
+            0 <= jj < N &&
+            grid[ii][jj] == grid[ii + 1][jj];
+      }
     }
   }
 
-lemma ReversePreservesMoreToMerge(grid: Grid)
-  requires ValidGrid(grid)
-  requires ValidValues(grid)
-  ensures MoreToMerge(grid) == MoreToMerge(Reverse(grid))
-{
-  // grid -> Reverse(grid)
-  if MoreToMerge(grid) {
-    if exists i, j ::
-        0 <= i < N && 0 <= j < N - 1 &&
-        grid[i][j] == grid[i][j + 1]
-    {
-      var i, j :|
-        0 <= i < N && 0 <= j < N - 1 &&
-        grid[i][j] == grid[i][j + 1];
-
-      assert 0 <= N - 2 - j < N - 1;
-      assert Reverse(grid)[i][N - 2 - j] == grid[i][j + 1];
-      assert Reverse(grid)[i][N - 1 - j] == grid[i][j];
-
-      assert exists ii, jj ::
-          ii == i &&
-          jj == N - 2 - j &&
-          0 <= ii < N &&
-          0 <= jj < N - 1 &&
-          Reverse(grid)[ii][jj] == Reverse(grid)[ii][jj + 1];
-    } else {
-      assert exists i, j {:trigger grid[i][j], grid[i + 1][j]} ::
-          0 <= i < N - 1 && 0 <= j < N &&
-          grid[i][j] == grid[i + 1][j];
-
-      var i, j :| 0 <= i < N - 1 && 0 <= j < N && grid[i][j] == grid[i + 1][j];
-
-      assert 0 <= N - 1 - j < N;
-      assert Reverse(grid)[i][N - 1 - j] == grid[i][j];
-      assert Reverse(grid)[i + 1][N - 1 - j] == grid[i + 1][j];
-
-      assert exists ii, jj {:trigger Reverse(grid)[ii][jj], Reverse(grid)[ii + 1][jj]} ::
-          ii == i &&
-          jj == N - 1 - j &&
-          0 <= ii < N - 1 &&
-          0 <= jj < N &&
-          Reverse(grid)[ii][jj] == Reverse(grid)[ii + 1][jj];
-    }
+  // two adjacent tiles with the same value in the same col
+  lemma ExistsVerticalMerge(grid: Grid) returns (i: int, j: int)
+    requires ValidGrid(grid)
+    requires ValidValues(grid)
+    requires exists i, j ::
+               twotilesadjacent(i, j, grid)
+    ensures 0 <= i < N - 1
+    ensures 0 <= j < N
+    ensures grid[i][j] == grid[i + 1][j]
+  {
+    // var i1, j1 :| 0 <= i1 < N - 1 && 0 <= j1 < N && grid[i1][j1] == grid[i1 + 1][j1];
+    var i1,j1:| twotilesadjacent(i1, j1, grid);
+    i, j := i1, j1;
   }
 
-  // Reverse(grid) -> grid
-  if MoreToMerge(Reverse(grid)) {
-    if exists i, j ::
-        0 <= i < N && 0 <= j < N - 1 &&
-        Reverse(grid)[i][j] == Reverse(grid)[i][j + 1]
-    {
-      var i, j :|
-        0 <= i < N && 0 <= j < N - 1 &&
-        Reverse(grid)[i][j] == Reverse(grid)[i][j + 1];
-
-      assert 0 <= N - 2 - j < N - 1;
-      assert Reverse(grid)[i][j] == grid[i][N - 1 - j];
-      assert Reverse(grid)[i][j + 1] == grid[i][N - 2 - j];
-
-      assert exists ii, jj ::
-          ii == i &&
-          jj == N - 2 - j &&
-          0 <= ii < N &&
-          0 <= jj < N - 1 &&
-          grid[ii][jj] == grid[ii][jj + 1];
-    } else {
-      assert exists i, j {:trigger Reverse(grid)[i][j], Reverse(grid)[i + 1][j]} ::
-          0 <= i < N - 1 && 0 <= j < N &&
-          Reverse(grid)[i][j] == Reverse(grid)[i + 1][j];
-
-      var i, j :| 0 <= i < N - 1 && 0 <= j < N && Reverse(grid)[i][j] == Reverse(grid)[i + 1][j];
-
-      assert 0 <= N - 1 - j < N;
-      assert Reverse(grid)[i][j] == grid[i][N - 1 - j];
-      assert Reverse(grid)[i + 1][j] == grid[i + 1][N - 1 - j];
-
-      assert exists ii, jj {:trigger grid[ii][jj], grid[ii + 1][jj]} ::
-          ii == i &&
-          jj == N - 1 - j &&
-          0 <= ii < N - 1 &&
-          0 <= jj < N &&
-          grid[ii][jj] == grid[ii + 1][jj];
-    }
-  }
-}
-
-  lemma TransposePreservesMoreToMerge(grid: Grid)
-  requires ValidGrid(grid)
-  requires ValidValues(grid)
-  ensures MoreToMerge(grid) == MoreToMerge(Transpose(grid))
-{
-  // grid -> Transpose(grid)
-  if MoreToMerge(grid) {
-    if exists i, j ::
-        0 <= i < N && 0 <= j < N - 1 &&
-        grid[i][j] == grid[i][j + 1]
-    {
-      var i, j :|
-        0 <= i < N && 0 <= j < N - 1 &&
-        grid[i][j] == grid[i][j + 1];
-
-      assert Transpose(grid)[j][i] == grid[i][j];
-      assert Transpose(grid)[j + 1][i] == grid[i][j + 1];
-
-      assert exists ii, jj {:trigger Transpose(grid)[ii][jj], Transpose(grid)[ii + 1][jj]} ::
-          ii == j &&
-          jj == i &&
-          0 <= ii < N - 1 &&
-          0 <= jj < N &&
-          Transpose(grid)[ii][jj] == Transpose(grid)[ii + 1][jj];
-    } else {
-      assert exists i, j {:trigger grid[i][j], grid[i + 1][j]} ::
-          0 <= i < N - 1 && 0 <= j < N &&
-          grid[i][j] == grid[i + 1][j];
-
-      var i, j :| 0 <= i < N - 1 && 0 <= j < N && grid[i][j] == grid[i + 1][j];
-
-      assert Transpose(grid)[j][i] == grid[i][j];
-      assert Transpose(grid)[j][i + 1] == grid[i + 1][j];
-
-      assert exists ii, jj ::
-          ii == j &&
-          jj == i &&
-          0 <= ii < N &&
-          0 <= jj < N - 1 &&
-          Transpose(grid)[ii][jj] == Transpose(grid)[ii][jj + 1];
-    }
+  predicate twotilesadjacent(i: int, j: int, grid: Grid)
+    requires ValidGrid(grid)
+  {
+    0 <= i < N - 1 && 0 <= j < N &&
+    grid[i][j] == grid[i + 1][j]
   }
 
-  // Transpose(grid) -> grid
-  if MoreToMerge(Transpose(grid)) {
-    if exists i, j ::
-        0 <= i < N && 0 <= j < N - 1 &&
-        Transpose(grid)[i][j] == Transpose(grid)[i][j + 1]
-    {
-      var i, j :|
-        0 <= i < N && 0 <= j < N - 1 &&
-        Transpose(grid)[i][j] == Transpose(grid)[i][j + 1];
-
-      assert Transpose(grid)[i][j] == grid[j][i];
-      assert Transpose(grid)[i][j + 1] == grid[j + 1][i];
-
-      assert exists ii, jj {:trigger grid[ii][jj], grid[ii + 1][jj]} ::
-          ii == j &&
-          jj == i &&
-          0 <= ii < N - 1 &&
-          0 <= jj < N &&
-          grid[ii][jj] == grid[ii + 1][jj];
-    } else {
-      assert exists i, j {:trigger Transpose(grid)[i][j], Transpose(grid)[i + 1][j]} ::
-          0 <= i < N - 1 && 0 <= j < N &&
-          Transpose(grid)[i][j] == Transpose(grid)[i + 1][j];
-
-      var i, j :| 0 <= i < N - 1 && 0 <= j < N && Transpose(grid)[i][j] == Transpose(grid)[i + 1][j];
-
-      assert Transpose(grid)[i][j] == grid[j][i];
-      assert Transpose(grid)[i + 1][j] == grid[j][i + 1];
-
-      assert exists ii, jj ::
-          ii == j &&
-          jj == i &&
-          0 <= ii < N &&
-          0 <= jj < N - 1 &&
-          grid[ii][jj] == grid[ii][jj + 1];
-    }
+  // two adjacent tiles with the same value in the same row
+  predicate twotilesadjacentrow(i: int, j: int, grid: Grid)
+    requires ValidGrid(grid)
+  {
+    0 <= i < N && 0 <= j < N - 1 &&
+    grid[i][j] == grid[i][j + 1]
   }
-}
-  // ============================================================
-  // 3. Combined game-state preservation
-  // ============================================================
+
+  lemma ExistsHorizontalMerge(grid: Grid) returns (i: int, j: int)
+    requires ValidGrid(grid)
+    requires ValidValues(grid)
+    requires exists i, j ::
+               twotilesadjacentrow(i, j, grid)
+    ensures 0 <= i < N
+    ensures 0 <= j < N - 1
+    ensures grid[i][j] == grid[i][j + 1]
+  {
+    var i1, j1 :| twotilesadjacentrow(i1, j1, grid);
+    i, j := i1, j1;
+  }
+
 
   lemma ReversePreservesLose(grid: Grid)
     requires ValidGrid(grid)
@@ -328,19 +271,6 @@ lemma ReversePreservesMoreToMerge(grid: Grid)
     ReversePreservesMoreToMerge(grid);
   }
 
-  lemma TransposePreservesLose(grid: Grid)
-    requires ValidGrid(grid)
-    requires ValidValues(grid)
-    ensures IsLose(grid) == IsLose(Transpose(grid))
-  {
-    TransposePreservesWin(grid);
-    TransposePreservesEmpty(grid);
-    TransposePreservesMoreToMerge(grid);
-  }
-
-  // ============================================================
-  // 4. Involution lemmas: applying twice gives back the original
-  // ============================================================
 
   lemma ReverseRowInvolution(row: seq<int>)
     requires |row| == N
@@ -380,6 +310,164 @@ lemma ReversePreservesMoreToMerge(grid: Grid)
 
     assert Reverse(Reverse(grid)) == grid;
   }
+
+
+  // -------------------transpose-----------------
+  // Transpose grid
+  function Transpose(grid: Grid): Grid
+    requires ValidGrid(grid)
+    ensures ValidGrid(Transpose(grid))
+    ensures forall i, j ::
+              0 <= i < N && 0 <= j < N ==>
+                Transpose(grid)[i][j] == grid[j][i]
+  {
+    seq(N, i requires 0 <= i < N =>
+      seq(N, j requires 0 <= j < N => grid[j][i]))
+  }
+
+
+  lemma TransposePreservesValues(grid: Grid)
+    requires ValidGrid(grid)
+    requires ValidValues(grid)
+    ensures ValidValues(Transpose(grid))
+  {
+    forall i, j | 0 <= i < N && 0 <= j < N
+      ensures Transpose(grid)[i][j] == 0 || IsPowerOfTwo(Transpose(grid)[i][j])
+    {
+      assert Transpose(grid)[i][j] == grid[j][i];
+    }
+  }
+
+  lemma TransposePreservesWin(grid: Grid)
+    requires ValidGrid(grid)
+    requires ValidValues(grid)
+    ensures HasWinTile(grid) == HasWinTile(Transpose(grid))
+  {
+    if HasWinTile(grid) {
+      var i, j :| 0 <= i < N && 0 <= j < N && grid[i][j] == 2048;
+      assert Transpose(grid)[j][i] == grid[i][j];
+      assert exists ii, jj :: 0 <= ii < N && 0 <= jj < N && Transpose(grid)[ii][jj] == 2048;
+    }
+
+    if HasWinTile(Transpose(grid)) {
+      var i, j :| 0 <= i < N && 0 <= j < N && Transpose(grid)[i][j] == 2048;
+      assert Transpose(grid)[i][j] == grid[j][i];
+      assert grid[j][i] == 2048;
+      assert exists ii, jj :: 0 <= ii < N && 0 <= jj < N && grid[ii][jj] == 2048;
+    }
+  }
+
+  lemma TransposePreservesEmpty(grid: Grid)
+    requires ValidGrid(grid)
+    requires ValidValues(grid)
+    ensures HasEmptyTile(grid) == HasEmptyTile(Transpose(grid))
+  {
+    if HasEmptyTile(grid) {
+      var i, j :| 0 <= i < N && 0 <= j < N && grid[i][j] == 0;
+      assert Transpose(grid)[j][i] == 0;
+      assert exists ii, jj :: 0 <= ii < N && 0 <= jj < N && Transpose(grid)[ii][jj] == 0;
+    }
+
+    if HasEmptyTile(Transpose(grid)) {
+      var i, j :| 0 <= i < N && 0 <= j < N && Transpose(grid)[i][j] == 0;
+      assert Transpose(grid)[i][j] == grid[j][i];
+      assert grid[j][i] == 0;
+      assert exists ii, jj :: 0 <= ii < N && 0 <= jj < N && grid[ii][jj] == 0;
+    }
+  }
+
+  lemma TransposePreservesMoreToMerge(grid: Grid)
+    requires ValidGrid(grid)
+    requires ValidValues(grid)
+    ensures MoreToMerge(grid) == MoreToMerge(Transpose(grid))
+  {
+    // grid -> Transpose(grid)
+    if MoreToMerge(grid) {
+      if exists i, j ::
+          0 <= i < N && 0 <= j < N - 1 &&
+          grid[i][j] == grid[i][j + 1]
+      {
+        var i, j :|
+          0 <= i < N && 0 <= j < N - 1 &&
+          grid[i][j] == grid[i][j + 1];
+
+        assert Transpose(grid)[j][i] == grid[i][j];
+        assert Transpose(grid)[j + 1][i] == grid[i][j + 1];
+
+        assert exists ii, jj {:trigger Transpose(grid)[ii][jj], Transpose(grid)[ii + 1][jj]} ::
+            ii == j &&
+            jj == i &&
+            0 <= ii < N - 1 &&
+            0 <= jj < N &&
+            Transpose(grid)[ii][jj] == Transpose(grid)[ii + 1][jj];
+      } else {
+        assert exists i, j {:trigger grid[i][j], grid[i + 1][j]} ::
+            0 <= i < N - 1 && 0 <= j < N &&
+            grid[i][j] == grid[i + 1][j];
+
+        var i, j :| 0 <= i < N - 1 && 0 <= j < N && grid[i][j] == grid[i + 1][j];
+
+        assert Transpose(grid)[j][i] == grid[i][j];
+        assert Transpose(grid)[j][i + 1] == grid[i + 1][j];
+
+        assert exists ii, jj ::
+            ii == j &&
+            jj == i &&
+            0 <= ii < N &&
+            0 <= jj < N - 1 &&
+            Transpose(grid)[ii][jj] == Transpose(grid)[ii][jj + 1];
+      }
+    }
+
+    // Transpose(grid) -> grid
+    if MoreToMerge(Transpose(grid)) {
+      if exists i, j ::
+          0 <= i < N && 0 <= j < N - 1 &&
+          Transpose(grid)[i][j] == Transpose(grid)[i][j + 1]
+      {
+        var i, j :|
+          0 <= i < N && 0 <= j < N - 1 &&
+          Transpose(grid)[i][j] == Transpose(grid)[i][j + 1];
+
+        assert Transpose(grid)[i][j] == grid[j][i];
+        assert Transpose(grid)[i][j + 1] == grid[j + 1][i];
+
+        assert exists ii, jj {:trigger grid[ii][jj], grid[ii + 1][jj]} ::
+            ii == j &&
+            jj == i &&
+            0 <= ii < N - 1 &&
+            0 <= jj < N &&
+            grid[ii][jj] == grid[ii + 1][jj];
+      } else {
+        assert exists i, j {:trigger Transpose(grid)[i][j], Transpose(grid)[i + 1][j]} ::
+            0 <= i < N - 1 && 0 <= j < N &&
+            Transpose(grid)[i][j] == Transpose(grid)[i + 1][j];
+
+        var i, j :| 0 <= i < N - 1 && 0 <= j < N && Transpose(grid)[i][j] == Transpose(grid)[i + 1][j];
+
+        assert Transpose(grid)[i][j] == grid[j][i];
+        assert Transpose(grid)[i + 1][j] == grid[j][i + 1];
+
+        assert exists ii, jj ::
+            ii == j &&
+            jj == i &&
+            0 <= ii < N &&
+            0 <= jj < N - 1 &&
+            grid[ii][jj] == grid[ii][jj + 1];
+      }
+    }
+  }
+
+  lemma TransposePreservesLose(grid: Grid)
+    requires ValidGrid(grid)
+    requires ValidValues(grid)
+    ensures IsLose(grid) == IsLose(Transpose(grid))
+  {
+    TransposePreservesWin(grid);
+    TransposePreservesEmpty(grid);
+    TransposePreservesMoreToMerge(grid);
+  }
+
 
   lemma TransposeInvolution(grid: Grid)
     requires ValidGrid(grid)
